src/aeq/map.lean
@@ -29,19 +29,19 @@ lemma map_core (H : eX ≡α⟨R⟩ eY)
       /- lam -/ X₁ Y₁ R x y eX eY a r,
     begin /- var -/
       intros X₂ Y₂ pX pY S F,
-      cases F x_R_y with _ H, cases H with _ x_S_y,
+      cases F x y x_R_y with _ H, cases H with _ x_S_y,
       exact var x_S_y
     end,
     begin /- app -/
       intros X₂ Y₂ pX pY S F,
-      exact app (rf pX pY @F) (re pX pY @F)
+      exact app (rf pX pY F) (re pX pY F)
     end,
     begin /- lam -/
       intros X₂ Y₂ pX pY S F,
       exact (lam $
         r (vset.prop_insert_of_subset _ pX)
           (vset.prop_insert_of_subset _ pY)
-          (λ x y, vrel.map.update _ _ @F))
+          (vrel.map.update x y F))
     end
   end
 
@@ -49,7 +49,7 @@ lemma map_core (H : eX ≡α⟨R⟩ eY)
 -- `S : X₂ ×ν Y₂`, as long as `X₁ ⊆ X₂` and `Y₁ ⊆ Y₂`.
 theorem map (pX : X₁ ⊆ X₂) (pY : Y₁ ⊆ Y₂)
 : R ⇒ν S → eX ≡α⟨R⟩ eY → exp.map pX eX ≡α⟨S⟩ exp.map pY eY :=
-  λ F H, map_core H pX pY @F
+  λ F H, map_core H pX pY F
 
 end /- section -/ --------------------------------------------------------------
 
@@ -59,11 +59,11 @@ variables {eX : exp X} {eY : exp Y} -- Expressions
 
 -- A wrapper for `map` in which the free variable sets do not change.
 theorem map.simple
-: (∀ {x : ν∈ X} {y : ν∈ Y}, ⟪x, y⟫ ∈ν R → ⟪x, y⟫ ∈ν S) → eX ≡α⟨R⟩ eY → eX ≡α⟨S⟩ eY :=
+: (∀ (x : ν∈ X) (y : ν∈ Y), ⟪x, y⟫ ∈ν R → ⟪x, y⟫ ∈ν S) → eX ≡α⟨R⟩ eY → eX ≡α⟨S⟩ eY :=
   assume F H,
-  have F' : R ⇒ν S, by apply vrel.map.simple; apply @F,
+  have F' : R ⇒ν S, by apply vrel.map.simple; apply F,
   exp.eq_of_map X eX ▸ exp.eq_of_map Y eY ▸
-    map (vset.prop_subset_refl X) (vset.prop_subset_refl Y) @F' H
+    map (vset.prop_subset_refl X) (vset.prop_subset_refl Y) F' H
 
 end /- section -/ --------------------------------------------------------------
 
